{"nbformat":4,"nbformat_minor":0,"metadata":{"colab":{"name":"LinearAlgebra.ipynb","provenance":[],"collapsed_sections":[]},"kernelspec":{"name":"python3","display_name":"Python 3"}},"cells":[{"cell_type":"markdown","metadata":{"id":"uUsJFA49xSLA","colab_type":"text"},"source":["#hy Learn Linear Algebra?\n","Why Learn Linear Algebra?\n","Welcome to the beautiful world of Linear Algebra. You would have learnt concepts such as\n","\n","Vectors\n","Matrices\n","Determinants\n","Eigen Values\n","Using Matrices, you would have numerically crunched formulae to get some numbers in your high school or college. Have you ever thought how all these concepts could be interpreted?\n","\n","This is the right course that will help you answer that.\n","\n","#Vectors Representation\n","Vectors Representation\n","Vectors in two dimension or 2-D are geometrically represented by a directed line segment between two points in space.\n","The starting point is called initial point, and the ending point is called terminal point.\n","Vectors are represented by lower case letters \\vec{u}​u​⃗​​ , \\vec{v}​v​⃗​​, \\vec{w}​w​⃗​​.\n","\n","#Components of a Vector\n","Components of a Vector\n","\"A vector can be represented as \\vec{v}​v​⃗​​ = (x1,y1). This means the initial point of the vector is the origin (0,0) and the terminal point is (x1,y1) in the coordinate axis.\"\n","\n","#Quick Facts\n","A vector with no length is called zero vector, denoted by \\vec{0}​0​⃗​​.\n","Negative of a given vector \\vec{v}​v​⃗​​ is denoted by \\vec{-v}​−v​⃗​​. It is the same vector in the opposite direction.\n","#Vector Addition\n","Vector Addition\n","If there are two vectors \\vec{u}​u​⃗​​ = (x1,y1) and \\vec{v}​v​⃗​​ = (x2,y2) in 2D space, the sum of the vectors is \\vec{w}​w​⃗​​ = \\vec{u}​u​⃗​​ + \\vec{v}​v​⃗​​ = (x1+x2 , y1+y2).\n","#Vector Difference\n","Vector Difference\n","If there are two vectors \\vec{u}​u​⃗​​ and \\vec{v}​v​⃗​​ in space, and if we want to find the difference between them. Then it can be denoted as \\vec{u}​u​⃗​​ - \\vec{v}​v​⃗​​ = \\vec{u}​u​⃗​​ + (\\vec{-v}​−v​⃗​​). It is the addition of one vector with the negative of the other vector.\n","\n","#Scaling Vectors\n","Scaling Vectors\n","Suppose we have a vector \\vec{v}​v​⃗​​ and a non zero scalar 's', then the scalar multiple of the vector denoted by s\\vec{v}​v​⃗​​ is a new vector whose length is s time \\vec{v}​v​⃗​​.\n","#Unit Basis Vectors\n","Unit Basis Vectors\n","From the above figure, \\hat{i}​i​^​​ and \\hat{j}​j​^​​ are vectors of length 1 pointing in the direction of X and Y axes respectively. They are referred to as Unit Basis vectors.\n","#Scaling Based on Unit Vectors\n","Scaling Based on Unit Vectors\n","Any point in space can be represented as a scaled version of the Unit Basis vectors.\n","A point (3,4) can be represented as \\hat{3i}​3i​^​​ + \\hat{4j}​4j​^​​.\n","\n","#Linear Combination of Vectors\n","When two vectors are scaled and added together, it is called a linear combination of two vectors.\n","Linear combination of vectors \\vec{u}​u​⃗​​ and \\vec{v}​v​⃗​​ is a\\vec{u}​u​⃗​​ + b\\vec{v}​v​⃗​​ , where a and b are scalars.\n","#Linear Combination of Vectors\n","When two vectors are scaled and added together, it is called a linear combination of two vectors.\n","Linear combination of vectors \\vec{u}​u​⃗​​ and \\vec{v}​v​⃗​​ is a\\vec{u}​u​⃗​​ + b\\vec{v}​v​⃗​​ , where a and b are scalars.\n","#Span of Vectors\n","Span of Vectors\n","From the previous card, take the linear combination example, a\\vec{u}​u​⃗​​ + b\\vec{v}​v​⃗​​ where \\vec{u}​u​⃗​​ and \\vec{v}​v​⃗​​ are vectors and a and b are scalars.\n","\n","If you let a and b take any arbitrary value in the space, then you can get all possible vectors in that space. This idea is called span of the vector\n","Span is said to be the set of all linear combination of vectors in a given subspace."]},{"cell_type":"markdown","metadata":{"id":"ZmfapffUyKdi","colab_type":"text"},"source":["#Defining Matrices\n","A matrix is an array of scalars from a field F arranged in m X n format. Each value in a matrix is known as an entry.\n","\n","Size of the array is written as m X n, where m and n are the number of rows and columns, respectively.\n","\n","Examples for Matrices -\n","\n","A = \\begin{pmatrix} 1 & 2 \\\\ 3 & 4 \\end{pmatrix}(​1​3​​​2​4​​)\n","\n","#Matrix Notation\n","Matrix Notation\n","The horizontal entries in a matrix are called rows.\n","The vertical entries are called columns.\n","\n","#Equality\n","Definition: Two matrices A and B are equal if and only if they have the same size and\n","\n","a_{ij}a​ij​​ = b_{ij}b​ij​​ for all i, j. (here i and j are the indices of the elements)\n","\n","Definition: If A is any matrix and \\alphaα \\in∈ F then the scalar multiplication B = \\alphaαA is defined by\n","\n","b_{ij}b​ij​​ = \\alphaα a_{ij}a​ij​​ for all i, j.\n","\n","Definition: If A and B are matrices of the same size then the sum A and B is defined by C = A + B, where\n","\n","c_{ij}c​ij​​ = a_{ij}a​ij​​ + b_{ij}b​ij​​ all i, j\n","\n","We can also compute the difference D = A − B by summing A and (−1)B D = A − B = A + (−1)B - matrix subtraction.\n","\n","Matrix addition “gets” multiple properties from the field F.\n","#Some Theorems to Ponder\n","A + B = B + A - commutivity\n","\n","A + (B + C) = (A + B) + C - associativity\n","\n","\\alphaα (A + B) = \\alphaαA + \\alphaαB - distributivity of a scalar\n","\n","If B = 0 (a matrix of all zeros) then A + B = A +0= A\n","\n","(\\alphaα + \\betaβ)A = \\alphaαA + \\betaβA\n","\n","\\alphaα(\\betaβA) = \\alpha\\betaαβA\n","\n","0A = 0\n","\n","\\alphaα 0 = 0\n","#Linear Transforms\n","Linear Transforms\n","A transformation takes in an Input and gives an Output.\n","\n","All lines must remain as lines.\n","Origin must remain fixed.\n","Definition: (Linear Transformation): A transformation (or mapping) T from a vector space S1 to a vector space S2, T: S1 → S2 is a linear transformation if:\n","\n","(i) T(\\vec{u}​u​⃗​​ + \\vec{v}​v​⃗​​) = T\\vec{u}​u​⃗​​ + T\\vec{v}​v​⃗​​ for all vectors \\vec{u}​u​⃗​​, \\vec{v}​v​⃗​​ in V1; and\n","\n","(ii) T(s\\vec{u}​u​⃗​​) = sT\\vec{u}​u​⃗​​ for all vectors \\vec{u}​u​⃗​​ in V1 and all scalars s.\n","#Some Facts About Linear Transformation\n","If L is a linear transformation, then L0 should be 0. (So if you find L0 not 0 , it means L is not a linear transformation.)\n","\n","• Any linear transformation T : R^nR​n​​ → R^mR​m​​ can be given by a matrix A of typem X n,\n","\n","T(\\vec{u}​u​⃗​​) = A\\vec{u}​u​⃗​​ for vectors \\vec{u}​u​⃗​​ in R^nR​n​​.\n","\n","#Examples of Linear Transformations\n","T = \\begin{bmatrix} a_1 \\\\ a_2 \\\\ a_3 \\\\ a_4 \\\\ a_5 \\\\ \\end{bmatrix}​⎣​⎢​⎢​⎢​⎢​⎢​⎢​⎡​​​a​1​​​a​2​​​a​3​​​a​4​​​a​5​​​​​​⎦​⎥​⎥​⎥​⎥​⎥​⎥​⎤​​ = \\begin{bmatrix} 1 & 2 & 3 & -2 & -1 \\\\ 0 & 3 & -1 & 4 & -3 \\\\ 1 & -1 & 2 & 4 & -3\\\\ 1 & -1 & 2 & 4 & -3\\\\ 1 & -1 & 2 & 4 & -3\\\\ \\end{bmatrix}​⎣​⎢​⎢​⎢​⎢​⎢​⎢​⎡​​​1​0​1​1​1​​​​2​3​−1​−1​−1​​​3​−1​2​2​2​​​−2​4​4​4​4​​​−1​−3​−3​−3​−3​​​⎦​⎥​⎥​⎥​⎥​⎥​⎥​⎤​​ \\cdot⋅ \\begin{bmatrix} a_1 \\\\ a_2 \\\\ a_3 \\\\ a_4 \\\\ a_5 \\\\ \\end{bmatrix}​⎣​⎢​⎢​⎢​⎢​⎢​⎢​⎡​​​a​1​​​a​2​​​a​3​​​a​4​​​a​5​​​​​​⎦​⎥​⎥​⎥​⎥​⎥​⎥​⎤​​\n","\n","Scaling expansion by a factor 3 T : R^3R​3​​ -> R^2R​2​​ with matrix \\begin{bmatrix} 3 & 0 & 0 \\\\ 0 & 3 & 0 \\\\ 0 & 0 & 3 \\end{bmatrix}​⎣​⎡​​​3​0​0​​​0​3​0​​​0​0​3​​​⎦​⎤​​\n","\n","Reflection in R^2R​2​​ through the x_2x​2​​ axis: matrix \\begin{bmatrix} -1 & 0 \\\\ 0 & 1 \\end{bmatrix}[​−1​0​​​0​1​​]\n","#xamples of Linear Transformations\n","T = \\begin{bmatrix} a_1 \\\\ a_2 \\\\ a_3 \\\\ a_4 \\\\ a_5 \\\\ \\end{bmatrix}​⎣​⎢​⎢​⎢​⎢​⎢​⎢​⎡​​​a​1​​​a​2​​​a​3​​​a​4​​​a​5​​​​​​⎦​⎥​⎥​⎥​⎥​⎥​⎥​⎤​​ = \\begin{bmatrix} 1 & 2 & 3 & -2 & -1 \\\\ 0 & 3 & -1 & 4 & -3 \\\\ 1 & -1 & 2 & 4 & -3\\\\ 1 & -1 & 2 & 4 & -3\\\\ 1 & -1 & 2 & 4 & -3\\\\ \\end{bmatrix}​⎣​⎢​⎢​⎢​⎢​⎢​⎢​⎡​​​1​0​1​1​1​​​​2​3​−1​−1​−1​​​3​−1​2​2​2​​​−2​4​4​4​4​​​−1​−3​−3​−3​−3​​​⎦​⎥​⎥​⎥​⎥​⎥​⎥​⎤​​ \\cdot⋅ \\begin{bmatrix} a_1 \\\\ a_2 \\\\ a_3 \\\\ a_4 \\\\ a_5 \\\\ \\end{bmatrix}​⎣​⎢​⎢​⎢​⎢​⎢​⎢​⎡​​​a​1​​​a​2​​​a​3​​​a​4​​​a​5​​​​​​⎦​⎥​⎥​⎥​⎥​⎥​⎥​⎤​​\n","\n","Scaling expansion by a factor 3 T : R^3R​3​​ -> R^2R​2​​ with matrix \\begin{bmatrix} 3 & 0 & 0 \\\\ 0 & 3 & 0 \\\\ 0 & 0 & 3 \\end{bmatrix}​⎣​⎡​​​3​0​0​​​0​3​0​​​0​0​3​​​⎦​⎤​​\n","\n","Reflection in R^2R​2​​ through the x_2x​2​​ axis: matrix \\begin{bmatrix} -1 & 0 \\\\ 0 & 1 \\end{bmatrix}[​−1​0​​​0​1​​]\n","\n","#Examples of Not Linear Transforms\n","L : R → R, L(x)L(x) = x^22x​2​​2\n","T : R^3R​3​​ → R^2R​2​​, T \\begin{bmatrix} a_1 \\\\ a_2 \\\\ a_3 \\\\ \\end{bmatrix}​⎣​⎢​⎢​⎡​​​a​1​​​a​2​​​a​3​​​​​​⎦​⎥​⎥​⎤​​ =\n","\\begin{bmatrix} 2a_2 - 5a_3 + 7a_4 + 6a_5 + 777 \\\\ -3a_1 + 4a_2 + 8a_3 - a_4 + a_5 \\end{bmatrix}[​2a​2​​−5a​3​​+7a​4​​+6a​5​​+777​−3a​1​​+4a​2​​+8a​3​​−a​4​​+a​5​​​​]\n","#Quote\n","If you are going to limit your dreams atleast\n","\n","\\lim\\limits_x f(x) = \\infty ​x​lim​​f(x)=∞\n","\n","tend them to infinity"]},{"cell_type":"markdown","metadata":{"id":"qvrskn8rKIYN","colab_type":"text"},"source":["#Defining Transpose\n","Defining Transpose\n","When a matrix A undergoes transpose operation, the rows of A become the columns of A transpose.\n","\n","Let A \\in∈ M m,n (F).\n","\n","Define the transpose of A, denoted by A^TA​T​​ , to be the n X m matrix with entries\n","{(A^T)}_{ij}(A​T​​)​ij​​ = a_{ji}a​ji​​ .\n","\n","#Example of Transpose\n","A = \\begin{bmatrix} 1 & 2 \\\\ 3 & 4 \\\\ 5 & 6 \\end{bmatrix}​⎣​⎡​​​1​3​5​​​2​4​6​​​⎦​⎤​​\n","\n","A^TA​T​​ = \\begin{bmatrix} 1 & 3 & 5 \\\\ 2 & 4 & 6 \\end{bmatrix}[​1​2​​​3​4​​​5​6​​]\n","\n","“The rows of A become the columns of A^TA​T​​, taken in the same order.”The following results are easy to prove.\n","\n","If A is of order m X n then A^TA​T​​ is n X m\n","\n","#Laws of transposes\n","(A^T)^T(A​T​​)​T​​ = AA\n","(A±B)^T = A^TA​T​​ ± B^TB​T​​\n","(cA)^T(cA)​T​​ = c A^TA​T​​\n","(AB)^T(AB)​T​​ = B^TB​T​​ A^TA​T​​\n","If AA is symmetric AA = A^TA​T​​\n","\n","#Matrix Vector Multiplication\n","Matrix Vector Multiplication\n","Matrix vector multiplication is performed in the above manner.\n","\n","#Matrix Multiplication\n","Matrix matrix multiplication is an extension of Matrix Vector Multiplication.\n","\n","Consider the matrix A = \\begin{pmatrix} 1 & 2 & 3 \\\\ 4 & 5 & 6 \\end{pmatrix}(​1​4​​​2​5​​​3​6​​)\n","\n","B = \\begin{pmatrix} 1 & 5 \\\\ 2 & -3 \\\\ 3 & -1 \\end{pmatrix}​⎝​⎛​​​1​2​3​​​5​−3​−1​​​⎠​⎞​​\n","\n","AB = \\begin{pmatrix} 14 & -4 \\\\ 32 & -1 \\end{pmatrix}(​14​32​​​−4​−1​​)\n","\n","Matrix multiplication is possible between matrices A and B only if the number of columns of A are equal to number of rows of B.\n","\n","#Properties of Matrix Multiplication\n","Consider two matrices A and B if AB and exists,then AB \\not =\\not= BA\n","\n","If A is square we can define A^1A​1​​ = A\n","A^2A​2​​ = AA\n","A^3A​3​​ = AAA\n","A^4A​4​​ = AAAA\n","\n","I = diag(1,...,1). If AA \\in∈ MM m,n (FF) then AI_nI​n​​ = A I_mI​m​​ A = A\n","\n","#Rules of Matrix Multiplication\n","Consider the following matrix A , B and C with order m X m\n","\n","A(BC) = (AB)C\n","A(B ± C) = AB ± AC and (A ± B)C = AC ± BC\n","AI = A and IA = A\n","c(AB) = (cA)B\n","A0 = 0 and 0B = 0\n","For A square marix A^rA​r​​ A^sA​s​​ = A^sA​s​​ A^rA​r​​ for all integers r, s ≥ 1.\n","\n","Fact: For given Matrices A,B,C If AC and BC are equal, it does not follow that A = B"]},{"cell_type":"markdown","metadata":{"id":"CZl_IR2AKngz","colab_type":"text"},"source":["#Matrix Determinant\n","Consider a matrix M of dimenstion 2 x 2 .\n","\n","M = \\begin{bmatrix} m_{11} & m_{12} \\\\ m_{21} & m_{22} \\end{bmatrix}[​m​11​​​m​21​​​​​m​12​​​m​22​​​​]\n","\n","The determinant of M is represented as det(M) or |M| The determinant is calculated in the following manner\n","\n","m_{11}m_{22}m​11​​m​22​​ - m_{21}m_{12}m​21​​m​12​​\n","\n","#Calculating the determinant\n","Conside the following matrix\n","\n","A = \\begin{pmatrix} 1 & 2 \\\\ 1 & 4 \\end{pmatrix}(​1​1​​​2​4​​) The determinant of A is represented as\n","\n","det(A) = \\begin{vmatrix} 1 & 2 \\\\ 1 & 4 \\end{vmatrix}​∣​∣​∣​∣​​​1​1​​​2​4​​​∣​∣​∣​∣​​ = 1 * 4 - 2 * 1 = 2\n","\n","#Minor of Matrix\n","Consider a Matrix A of dimension 3 x 3 .\n","\n","A = \\begin{bmatrix} 1 & 2 & 3 \\\\ 4 & 5 & 6 \\\\ 7 & 8 & 9 \\end{bmatrix}​⎣​⎡​​​1​4​7​​​2​5​8​​​3​6​9​​​⎦​⎤​​\n","\n","The minor M_{12}M​12​​ is the determinant of the matrix obtained after eliminating first row and second column.\n","\n","M_{12}M​12​​ = \\begin{vmatrix} 4 & 6 \\\\ 7 & 9 \\end{vmatrix}​∣​∣​∣​∣​​​4​7​​​6​9​​​∣​∣​∣​∣​​ = 36 - 42 = -6\n","\n","The minor M_{22}M​22​​ is the determinant of the matrix obtained after eliminating second row and second column.\n","\n","M_{22}M​22​​ = \\begin{vmatrix} 1 & 3 \\\\ 7 & 9 \\end{vmatrix}​∣​∣​∣​∣​​​1​7​​​3​9​​​∣​∣​∣​∣​​ = 9 - 21 = -12\n","\n","#Cofactor Matrix\n","The cofactor C_{i,j}C​i,j​​ of a Matrix A is defined by the relationship C_{i,j}C​i,j​​ = (-1)^{i+j}(−1)​i+j​​ M_{i,j}M​i,j​​\n","\n","Where M_{i,j}M​i,j​​ is the Minor.\n","\n","Consider the Matrix A = \\begin{pmatrix} 1 & 2 & 3 \\\\ 4 & 5 & 6 \\\\ 7 & 8 & 9 \\end{pmatrix}​⎝​⎛​​​1​4​7​​​2​5​8​​​3​6​9​​​⎠​⎞​​\n","\n","M_{1,2}M​1,2​​ = -6\n","\n","C_{1,2}C​1,2​​ = (-1)^{1+2}(−1)​1+2​​ M_{1,2}M​1,2​​ = -1 . -6 = 6\n","\n","#Calculating Determinant from Co factor\n","Calculating Determinant from Co-factor\n","\n","Given a square Matrix P and its cofactors C_{i,j}C​i,j​​ , the determinant can be obtained by co-factor expansion method.\n","\n","Steps\n","\n","Choose a specific Row or Column of the matrix P\n","Multiply each element p_{i,j}p​i,j​​ chosen with its respective co-factor C_{i,j}C​i,j​​ and add the results\n","\n","#Determinant of a Matrix\n","For a given 3 x 3 matrix the determinant would be\n","\n","det A = a_{11}a​11​​ C_{11}C​11​​ + a_{12}a​12​​ C_{12}C​12​​ + a_{13}a​13​​ C_{13}C​13​​\n","\n","The determinant can also be calculated by choosing any other row or column\n","\n","det A = a_{21}a​21​​ C_{21}C​21​​ + a_{22}a​22​​ C_{22}C​22​​ + a_{23}a​23​​ C_{23}C​23​​\n","\n","Consider the matrix\n","\n","A = \\begin{bmatrix} 2 & 1 & 3 \\\\ 1 & 0 & 2 \\\\ 2 & 0 & -2 \\end{bmatrix}A=​⎣​⎡​​​2​1​2​​​1​0​0​​​3​2​−2​​​⎦​⎤​​\n","\n","Applying Co-factor expansion\n","\n","a_{11}a​11​​ = 2 a_{12}a​12​​ = 1 a_{13}a​13​​ = 3\n","\n","C_{11}C​11​​ = (-1)^{1+1}(−1)​1+1​​ M_{11}M​11​​ = 1 \\begin{vmatrix} 0 & 2 \\\\ 0 & -2 \\end{vmatrix}​∣​∣​∣​∣​​​0​0​​​2​−2​​​∣​∣​∣​∣​​ = 0\n","\n","C_{12}C​12​​ = (-1)^{1+2}(−1)​1+2​​ M_{12}M​12​​ = -1 \\begin{vmatrix} 1 & 2 \\\\ 2 & -2\\end{vmatrix}​∣​∣​∣​∣​​​1​2​​​2​−2​​​∣​∣​∣​∣​​ = 6\n","\n","C_{13}C​13​​ = (-1)^{1+3}(−1)​1+3​​ M_{13}M​13​​ = 1 \\begin{vmatrix} 1 & 0 \\\\ 2 & 0 \\end{vmatrix}​∣​∣​∣​∣​​​1​2​​​0​0​​​∣​∣​∣​∣​​ = 0\n","\n","det A = 2 x 0 + 6 x 1 + 3 x 0 = 6\n","\n","#Invertible Matrices\n","Inverse of a Matrix Let A be a square matrix of order n.\n","\n","A square matrix B is said to be a left inverse of A if\n","BABA = I_nI​n​​\n","A square matrix C is called a right inverse of A, if\n","ACAC = I_nI​n​​\n","A matrix A is said to be invertible(or is said to have an inverse)if there exists a matrix B such that\n","ABAB = BABA = I_nI​n​​\n","Where I_nI​n​​ is the identity matrix of order n\n","\n","#Properties of Invertibility\n","(A^{-1})^{-1}(A​−1​​)​−1​​ = AA\n","\n","(AB)^{-1}(AB)​−1​​ = B^{-1} A^{-1}B​−1​​A​−1​​\n","\n","(A^t)^{-1} = (A^{-1})^t(A​t​​)​−1​​=(A​−1​​)​t​​\n","\n","#Row Column and Null Space\n","For a given vector AA = (-1 ,1,3)(−1,1,3) , null space consists of the solution to AxAx = 00\n","\n","Consider a Matrix A\n","\n","A = \\begin{pmatrix} 1 & 2 & 3 \\\\ 4 & 5 & 6 \\\\ 7 & 8 & 9 \\end{pmatrix}​⎝​⎛​​​1​4​7​​​2​5​8​​​3​6​9​​​⎠​⎞​​\n","\n","Row Space of A is span {(1,2,3)^t ,(4,5,6)^t , (7,8,9)^t}^1(1,2,3)​t​​,(4,5,6)​t​​,(7,8,9)​t​​​1​​\n","\n","Column Space of A is span {\\begin{pmatrix} 1 \\\\ 4 \\\\ 7 \\end{pmatrix}​⎝​⎛​​​1​4​7​​​⎠​⎞​​ ,\\begin{pmatrix} 2 \\\\ 5 \\\\ 8 \\end{pmatrix}​⎝​⎛​​​2​5​8​​​⎠​⎞​​ ,\\begin{pmatrix} 3 \\\\ 6 \\\\ 9 \\end{pmatrix}​⎝​⎛​​​3​6​9​​​⎠​⎞​​}"]},{"cell_type":"markdown","metadata":{"id":"YyXmMf92K_CR","colab_type":"text"},"source":["#Dot Product Definition\n","Dot Product Definition\n","The scalar dot product of two vectors xx = (x_1,x_2,...x_n)(x​1​​,x​2​​,...x​n​​) and yy = (y_1,y_2,...y_n)(y​1​​,y​2​​,...y​n​​) is given by x \\cdot yx⋅y = x_1y_1x​1​​y​1​​ + x_2y_2x​2​​y​2​​ + x_3y_3x​3​​y​3​​ + ... x_ky_kx​k​​y​k​​ = \\displaystyle\\sum_{k=1}^n x_ky_k​k=1​∑​n​​x​k​​y​k​​\n","\n","Dot Product Example\n","Consider the following Example\n","\n","x = (2,-1) y = (3,1)\n","\n","x.y = 2.3 + -1.1 = 6 -1 = 5 .\n","\n","#Dot Product Properties\n","x \\cdot x >= 0x⋅x>=0 this is the positivity property.\n","x \\cdot x = 0x⋅x=0 only when x = 0x=0\n","x \\cdot y = y \\cdot xx⋅y=y⋅x This is the Symmetry Property\n","(x+y) \\cdot z = x \\cdot z + y \\cdot z(x+y)⋅z=x⋅z+y⋅z Distributive Law\n","(rx) \\cdot y = r(x \\cdot y)(rx)⋅y=r(x⋅y) homogeneity\n","\n","#Vector Cross Product\n","Vector Cross Product\n","The cross product x is an operation that takes two vectors \\vec{u}​u​⃗​​ and \\vec{v}​v​⃗​​ in space and determines another vector \\vec{u}​u​⃗​​ x \\vec{v}​v​⃗​​ in space.\n","\n","The geometric interpretation is the area of parallelogram formed by the two vectors \\vec{u}​u​⃗​​ and \\vec{v}​v​⃗​​ .\n","\n","#Determining the Cross Product\n","Consider two vectors \\vec{u}​u​⃗​​ = (u_1,u_2,u_3)(u​1​​,u​2​​,u​3​​) and \\vec{v}​v​⃗​​ = (v_1,v_2,v_3)(v​1​​,v​2​​,v​3​​)\n","\n","\\vec{u}​u​⃗​​ x \\vec{v}​v​⃗​​ = (u_2v_3u​2​​v​3​​ − u_3v_2u​3​​v​2​​) \\hat{i}​i​^​​ + (u_3v_1u​3​​v​1​​ − u_1v_3u​1​​v​3​​) \\hat{j}​j​^​​ + (u_1 v_2u​1​​v​2​​ − u_2v_1u​2​​v​1​​) \\hat{k}​k​^​​\n","\n","\\vec{u}​u​⃗​​ x \\vec{v}​v​⃗​​ = \\begin{vmatrix} \\hat{i} & \\hat{j} & \\hat{k} \\\\ u_1 & u_2 & u_3 \\\\ v_1 & v_2 & v_3 \\end{vmatrix}​∣​∣​∣​∣​∣​∣​​​​i​^​​​u​1​​​v​1​​​​​​j​^​​​u​2​​​v​2​​​​​​k​^​​​u​3​​​v​3​​​​​∣​∣​∣​∣​∣​∣​​\n","\n","#Properties of Cross Product\n","\\vec{v}​v​⃗​​ x \\vec{u}​u​⃗​​ = −(\\vec{u}​u​⃗​​ x \\vec{v}​v​⃗​​)\n","\n","\\vec{u}​u​⃗​​ x \\vec{u}​u​⃗​​ = 00\n","\n","Cross product distributes over addition and subtraction\n","\n","00 x \\vec{u}​u​⃗​​ = 00 = \\vec{u}​u​⃗​​ x 00\n","\n","c(\\vec{u}​u​⃗​​ × \\vec{v}​v​⃗​​) = (c\\vec{u}​u​⃗​​) × \\vec{v}​v​⃗​​ = \\vec{u}​u​⃗​​ × (c\\vec{v}​v​⃗​​)\n","\n","#Change of Basis\n","Change of Basis\n","We usually go for unit vectors as basis to construct other vectors in space.\n","When we go with other vectors as basis , it is called change of basis.\n","\n"]},{"cell_type":"markdown","metadata":{"id":"HL01mk8eOcNh","colab_type":"text"},"source":["#Eigenvectors and eigenvalues\n","For a matrix A , if any vector \\vec{x}​x​⃗​​ <> 0 satisfies the equation Ax = \\lambda xAx=λx then\n","\n","\\lambdaλ is the eigenvalue of Matrix A .\n","\n","xx is eigenvector of A corresponding to eigenvalue \\lambdaλ .\n","\n","#Calculating the value and vector\n","Consider the matrix\n","\n","AA = \\begin{pmatrix} 2 & 3 \\\\ 3 & 2 \\end{pmatrix}(​2​3​​​3​2​​)\n","\n","xx = \\begin{pmatrix} 1 \\\\ 1 \\end{pmatrix}(​1​1​​)\n","\n","AxAx = \\begin{pmatrix} 5 \\\\ 5 \\end{pmatrix}(​5​5​​) = 5x5x\n","\n","\\lambdaλ = 5 is eigenvalue of A\n","\n","x is an eigen vector corresponding to eigen value\n","#Applications\n","Some prominent applications of Eigen Values and Eigen Vectors\n","\n","Google's Page Ranking Algorithm\n","Singular Value Decomposition\n","Principle Component Analysis"]},{"cell_type":"markdown","metadata":{"id":"g3beRoBYOwzc","colab_type":"text"},"source":["#SVD Explained\n","SVD Explained\n","The above image explains how a given matrix can be disintegrated into 3 different matrices by preserving their properties.\n","\n","#Applications\n","Singular Value Decomposition can be used for\n","\n","Solving Linear Equations\n","Dimension Reduction for Machine Learning Problems\n","Image Compression\n","\n","Principle Component Analysis\n","PCA is a very important dimension reduction technique .\n","\n","It has very good applications in Machine Learning.\n","\n","The following videos will explain PCA in detail.\n","\n","Applications of PCA\n","PCA is used for\n","\n","Dimension Reduction of Feature Vectors in Machine Learning Problems"]}]}